

**2017 AP<sup>®</sup> CALCULUS BC FREE-RESPONSE QUESTIONS**

$$\begin{aligned}f(0) &= 0 \\f'(0) &= 1 \\f^{(n+1)}(0) &= -n \cdot f^{(n)}(0) \text{ for all } n \geq 1\end{aligned}$$

6. A function  $f$  has derivatives of all orders for  $-1 < x < 1$ . The derivatives of  $f$  satisfy the conditions above. The Maclaurin series for  $f$  converges to  $f(x)$  for  $|x| < 1$ .

(a) Show that the first four nonzero terms of the Maclaurin series for  $f$  are  $x - \frac{x^2}{2} + \frac{x^3}{3} - \frac{x^4}{4}$ , and write the general term of the Maclaurin series for  $f$ .

(b) Determine whether the Maclaurin series described in part (a) converges absolutely, converges conditionally, or diverges at  $x = 1$ . Explain your reasoning.

(c) Write the first four nonzero terms and the general term of the Maclaurin series for  $g(x) = \int_0^x f(t) \, dt$ .

(d) Let  $P_n\left(\frac{1}{2}\right)$  represent the  $n$ th-degree Taylor polynomial for  $g$  about  $x = 0$  evaluated at  $x = \frac{1}{2}$ , where  $g$  is the function defined in part (c). Use the alternating series error bound to show that

$$\left| P_4\left(\frac{1}{2}\right) - g\left(\frac{1}{2}\right) \right| < \frac{1}{500}.$$

---

**STOP**  
**END OF EXAM**

**AP<sup>®</sup> CALCULUS BC**  
**2017 SCORING GUIDELINES**

**Question 6**

(a)  $f(0) = 0$

$$f'(0) = 1$$

$$f''(0) = -1(1) = -1$$

$$f'''(0) = -2(-1) = 2$$

$$f^{(4)}(0) = -3(2) = -6$$

The first four nonzero terms are

$$0 + 1x + \frac{-1}{2!}x^2 + \frac{2}{3!}x^3 + \frac{-6}{4!}x^4 = x - \frac{x^2}{2} + \frac{x^3}{3} - \frac{x^4}{4}.$$

The general term is  $\frac{(-1)^{n+1}x^n}{n}$ .

(b) For  $x = 1$ , the Maclaurin series becomes  $\sum_{n=1}^{\infty} \frac{(-1)^{n+1}}{n}$ .

The series does not converge absolutely because the harmonic series diverges.

The series alternates with terms that decrease in magnitude to 0, and therefore the series converges conditionally.

(c) 
$$\int_0^x f(t) dt = \int_0^x \left( t - \frac{t^2}{2} + \frac{t^3}{3} - \frac{t^4}{4} + \cdots + \frac{(-1)^{n+1}t^n}{n} + \cdots \right) dt$$

$$= \left[ \frac{t^2}{2} - \frac{t^3}{3 \cdot 2} + \frac{t^4}{4 \cdot 3} - \frac{t^5}{5 \cdot 4} + \cdots + \frac{(-1)^{n+1}t^{n+1}}{(n+1)n} + \cdots \right]_{t=0}^{t=x}$$

$$= \frac{x^2}{2} - \frac{x^3}{6} + \frac{x^4}{12} - \frac{x^5}{20} + \cdots + \frac{(-1)^{n+1}x^{n+1}}{(n+1)n} + \cdots$$

(d) The terms alternate in sign and decrease in magnitude to 0. By the alternating series error bound, the error  $\left| P_4\left(\frac{1}{2}\right) - g\left(\frac{1}{2}\right) \right|$  is bounded by the magnitude of the first unused term,  $\left| -\frac{(1/2)^5}{20} \right|$ .

Thus,  $\left| P_4\left(\frac{1}{2}\right) - g\left(\frac{1}{2}\right) \right| \leq \left| -\frac{(1/2)^5}{20} \right| = \frac{1}{32 \cdot 20} < \frac{1}{500}.$

$$3 : \begin{cases} 1 : f''(0), f'''(0), \text{ and } f^{(4)}(0) \\ 1 : \text{verify terms} \\ 1 : \text{general term} \end{cases}$$

2 : converges conditionally with reason

$$3 : \begin{cases} 1 : \text{two terms} \\ 1 : \text{remaining terms} \\ 1 : \text{general term} \end{cases}$$

1 : error bound